Propagate state with reachability to Recombination
Most of the changes are of the same straightforward sort as those
needed in CS. The operation to merge two reachability sets along the
lines of an interface is only a stub, and the corresponding symmetry
lemma admitted, but otherwise everything looks simple.

Intermediate/Recombination.v
@@ -50,10 +50,16 @@ Section Merge.
   Definition merge_pcs (pc pc'' : Pointer.t) : Pointer.t :=
     if Pointer.component pc \in domm ip then pc else pc''.
 
+  (* TODO: [DynShare] CS.reach_addr should probably live outside CS. The actual
+     definition is probably similar to those for the other components of the
+     program state. *)
+  Definition merge_addrs (addrs addrs'' : CS.reach_addr) : CS.reach_addr :=
+    addrs.
+
   Definition merge_states (state state'' : CS.state) : CS.state :=
-    let '(s, m, r, pc) := state in
-    let '(s'', m'', r'', pc'') := state'' in
-    (merge_stacks s s'', merge_memories m m'', merge_registers r r'' pc, merge_pcs pc pc'').
+    let '(s, m, r, pc, addrs) := state in
+    let '(s'', m'', r'', pc'', addrs'') := state'' in
+    (merge_stacks s s'', merge_memories m m'', merge_registers r r'' pc, merge_pcs pc pc'', merge_addrs addrs addrs'').
 
   Lemma merge_frames_program frame frame'' :
     Pointer.component frame \in domm ip ->
@@ -106,9 +112,13 @@ Section Merge.
     else
       CS.state_pc s''.
 
+  (* TODO: [DynShare] *)
+  Definition merge_states_addrs s (s'' : CS.state) :=
+    CS.state_addrs s.
+
   Lemma merge_states_unfold s s'' :
     merge_states s s'' =
-    (merge_states_stack s s'', merge_states_mem s s'', merge_states_regs s s'', merge_states_pc s s'').
+    (merge_states_stack s s'', merge_states_mem s s'', merge_states_regs s s'', merge_states_pc s s'', merge_states_addrs s s'').
   Proof. now CS.unfold_states. Qed.
 End Merge.
 
@@ -260,7 +270,7 @@ Section Mergeable.
     merge_states_regs ip s s'' = CS.state_regs s.
   Proof.
     intros Hcomp Hmerg.
-    destruct s as [[[stack mem] reg] pc]; destruct s'' as [[[stack'' mem''] reg''] pc''].
+    destruct s as [[[[stack mem] reg] pc] addrs]; destruct s'' as [[[[stack'' mem''] reg''] pc''] addrs''].
     unfold merge_states_regs. simpl.
     unfold merge_registers.
     CS.simplify_turn.
@@ -278,7 +288,7 @@ Section Mergeable.
     merge_states_regs ip s s'' = CS.state_regs s''.
   Proof.
     intros Hcomp Hmerg.
-    destruct s as [[[stack mem] reg] pc]; destruct s'' as [[[stack'' mem''] reg''] pc''].
+    destruct s as [[[[stack mem] reg] pc] addrs]; destruct s'' as [[[[stack'' mem''] reg''] pc''] addrs''].
     unfold merge_states_regs. simpl.
     unfold merge_registers.
     unfold CS.is_program_component, CS.is_context_component, turn_of, CS.state_turn in Hcomp.
@@ -298,7 +308,7 @@ Section Mergeable.
     merge_states_pc ip s s'' = CS.state_pc s.
   Proof.
     intros Hcomp Hmerg.
-    destruct s as [[[stack mem] reg] pc]; destruct s'' as [[[stack'' mem''] reg''] pc''].
+    destruct s as [[[[stack mem] reg] pc] addrs]; destruct s'' as [[[[stack'' mem''] reg''] pc''] addrs''].
     unfold merge_states_pc. simpl.
     unfold merge_pcs.
     unfold CS.is_program_component, CS.is_context_component, turn_of, CS.state_turn in Hcomp.
@@ -316,7 +326,7 @@ Section Mergeable.
     merge_states_pc ip s s'' = CS.state_pc s''.
   Proof.
     intros Hcomp Hmerg.
-    destruct s as [[[stack mem] reg] pc]; destruct s'' as [[[stack'' mem''] reg''] pc''].
+    destruct s as [[[[stack mem] reg] pc] addrs]; destruct s'' as [[[[stack'' mem''] reg''] pc''] addrs''].
     unfold merge_states_pc. simpl.
     unfold CS.is_program_component, CS.is_context_component, turn_of, CS.state_turn in Hcomp.
     inversion Hmerg as [_ _ _ _ _ _ _ Hmergeable_ifaces _ _ _ _ _ _ _ _].
@@ -333,7 +343,7 @@ Section Mergeable.
     CS.is_program_component s ic ->
     mergeable_states s s'' ->
     merge_states ip ic s s'' =
-    (merge_states_stack ip s s'', merge_states_mem ip ic s s'', CS.state_regs s, CS.state_pc s).
+    (merge_states_stack ip s s'', merge_states_mem ip ic s s'', CS.state_regs s, CS.state_pc s, CS.state_addrs s (* [DynShare] TODO *)).
   Proof.
     intros Hcomp Hmerg.
     rewrite merge_states_unfold.
@@ -346,7 +356,7 @@ Section Mergeable.
     CS.is_context_component s ic ->
     mergeable_states s s'' ->
     merge_states ip ic s s'' =
-    (merge_states_stack ip s s'', merge_states_mem ip ic s s'', CS.state_regs s'', CS.state_pc s'').
+    (merge_states_stack ip s s'', merge_states_mem ip ic s s'', CS.state_regs s'', CS.state_pc s'', CS.state_addrs s (* [DynShare] TODO *)).
   Proof.
     intros Hcomp Hmerg.
     rewrite merge_states_unfold.
@@ -388,8 +398,8 @@ Section Mergeable.
     CS.is_program_component s   ic ->
     CS.is_program_component s'' ic.
   Proof.
-    destruct s   as [[[? ?] ?] pc  ].
-    destruct s'' as [[[? ?] ?] pc''].
+    destruct s   as [[[[? ?] ?] pc  ] ?].
+    destruct s'' as [[[[? ?] ?] pc''] ?].
     unfold CS.is_program_component, CS.is_context_component, turn_of, CS.state_turn.
     intros Hmerge Hpc.
     pose proof mergeable_states_pc_same_component Hmerge as Hcomp. simpl in Hcomp.
@@ -403,7 +413,7 @@ Section Mergeable.
   Proof.
     intros Hmerg.
     unfold CS.is_program_component, CS.is_context_component, turn_of, CS.state_turn.
-    destruct s1 as [[[stack1 mem1] reg1] pc1]; destruct s2 as [[[stack2 mem2] reg2] pc2].
+    destruct s1 as [[[[stack1 mem1] reg1] pc1] addrs1]; destruct s2 as [[[[stack2 mem2] reg2] pc2] addrs2].
     pose proof mergeable_states_pc_same_component Hmerg as Hpc; simpl in Hpc.
     rewrite <- Hpc; clear Hpc.
     inversion Hmerg as [? ? ? _ _ _ _ [[_ Hdisj] _] _ _ _ _ Hini Hini'' Hstar Hstar''].
@@ -419,7 +429,7 @@ Section Mergeable.
   Proof.
     intros Hmerg.
     unfold CS.is_program_component, CS.is_context_component, turn_of, CS.state_turn.
-    destruct s as [[[stack mem] reg] pc]; destruct s'' as [[[stack'' mem''] reg''] pc''].
+    destruct s as [[[[stack mem] reg] pc] addrs]; destruct s'' as [[[[stack'' mem''] reg''] pc''] addrs''].
     pose proof mergeable_states_pc_same_component Hmerg as Hpc; simpl in Hpc.
     rewrite <- Hpc.
     inversion Hmerg as [s0 _ t
@@ -461,16 +471,16 @@ Section Mergeable.
       apply mergeable_states_program_to_context in Hcc; try assumption.
     unfold CS.is_context_component, turn_of, CS.state_turn in Hcc.
     rewrite (mergeable_states_pc_same_component Hmerge).
-    now destruct s'' as [[[? ?] ?] ?].
+    now destruct s'' as [[[[? ?] ?] ?] ?].
   Qed.
 
-  Lemma mergeable_states_program_component_domm mem gps regs pc s'' :
-    mergeable_states (mem, gps, regs, pc) s'' ->
-    CS.is_program_component (mem, gps, regs, pc) ic ->
+  Lemma mergeable_states_program_component_domm mem gps regs pc addrs s'' :
+    mergeable_states (mem, gps, regs, pc, addrs) s'' ->
+    CS.is_program_component (mem, gps, regs, pc, addrs) ic ->
     Pointer.component pc \in domm ip.
   Proof.
     intros Hmerge Hcomp.
-    change pc with (CS.state_pc (mem, gps, regs, pc)).
+    change pc with (CS.state_pc (mem, gps, regs, pc, addrs)).
     eapply is_program_component_pc_in_domm; last eassumption; assumption.
   Qed.
 
@@ -487,19 +497,19 @@ Section Mergeable.
       mergeable_stack (frame :: gps) (frame'' :: gps'').
 
   Lemma mergeable_states_mergeable_stack
-        gps1   mem1   regs1   pc1
-        gps1'' mem1'' regs1'' pc1'' :
-    mergeable_states (gps1  , mem1  , regs1  , pc1  )
-                     (gps1'', mem1'', regs1'', pc1'') ->
+        gps1   mem1   regs1   pc1   addrs1
+        gps1'' mem1'' regs1'' pc1'' addrs1'' :
+    mergeable_states (gps1  , mem1  , regs1  , pc1  , addrs1  )
+                     (gps1'', mem1'', regs1'', pc1'', addrs1'') ->
     mergeable_stack gps1 gps1''.
   Proof.
     intros Hmerg.
     inversion Hmerg
       as [_ _ _ Hwfp Hwfc Hwfp' Hwfc' Hmergeable_ifaces
           Hifacep Hifacec Hprog_is_closed Hprog_is_closed' _ _ _ _].
-    remember (gps1, mem1, regs1, pc1) as s1.
-    remember (gps1'', mem1'', regs1'', pc1'') as s1''.
-    revert gps1 mem1 regs1 pc1 gps1'' mem1'' regs1'' pc1'' Heqs1 Heqs1''.
+    remember (gps1, mem1, regs1, pc1, addrs1) as s1.
+    remember (gps1'', mem1'', regs1'', pc1'', addrs1'') as s1''.
+    revert gps1 mem1 regs1 pc1 addrs1 gps1'' mem1'' regs1'' pc1'' addrs1'' Heqs1 Heqs1''.
     induction Hmerg as [ s1 s1'' Hini Hini''
                        | s1 s2 s1'' Hmerg Hstep IH
                        | s1 s1'' s2'' Hmerg Hstep'' IH
@@ -520,7 +530,7 @@ Section Mergeable.
         try match goal with
         | Heq: _ = (_, _, _, _) |- _ => inversion Heq; subst; now eapply IH
         end.
-    - intros gps2 mem2 regs2 pc2 gps2'' mem2'' regs2'' pc2'' Heqs2 Heqs2''; subst.
+    - intros gps2 mem2 regs2 pc2 addrs2 gps2'' mem2'' regs2'' pc2'' addrs2'' Heqs2 Heqs2''; subst.
       (* Note: do not try to do:
          inversion Hstep; inversion Hstep''; try congruence.
          as it generates 13*13 = subgoals before discarding the
@@ -538,15 +548,15 @@ Section Mergeable.
         rewrite Pointer.inc_preserves_component.
         unfold sem, prog in *; simpl in *; eapply CS.star_pc_domm; try eassumption.
         now eapply IH.
-      + specialize (IH _ _ _ _ _ _ _ _ eq_refl eq_refl);
+      + specialize (IH _ _ _ _ _ _ _ _ _ _ eq_refl eq_refl);
           now inversion IH.
   Qed.
 
   Lemma mergeable_states_cons_domm
-        frame1   gps1   mem1   regs1   pc1
-        frame1'' gps1'' mem1'' regs1'' pc1'' :
-    mergeable_states (frame1   :: gps1  , mem1  , regs1  , pc1  )
-                     (frame1'' :: gps1'', mem1'', regs1'', pc1'') ->
+        frame1   gps1   mem1   regs1   pc1   addrs1
+        frame1'' gps1'' mem1'' regs1'' pc1'' addrs1'' :
+    mergeable_states (frame1   :: gps1  , mem1  , regs1  , pc1  , addrs1  )
+                     (frame1'' :: gps1'', mem1'', regs1'', pc1'', addrs1'') ->
     Pointer.component frame1 = Pointer.component frame1''.
   Proof.
     intros Hmerge.
@@ -565,8 +575,8 @@ Section Mergeable.
   exists mem,
     Memory.store (CS.state_mem s) ptr v = Some mem.
   Proof.
-    destruct s as [[[gps mem] regs] pc].
-    destruct s'' as [[[gps'' mem''] regs''] pc''].
+    destruct s as [[[[gps mem] regs] pc] addrs].
+    destruct s'' as [[[[gps'' mem''] regs''] pc''] addrs''].
     destruct ptr as [[C b] o].
     unfold Memory.store, merge_states, merge_states_mem, merge_memories.
     intros Hmerge_ifaces Hdomm Hcomp.
@@ -590,8 +600,8 @@ Section Mergeable.
   exists mem ptr,
     Memory.alloc (CS.state_mem s) (CS.state_component s) size = Some (mem, ptr).
   Proof.
-    destruct s as [[[gps mem] regs] pc].
-    destruct s'' as [[[gps'' mem''] regs''] pc''].
+    destruct s as [[[[gps mem] regs] pc] addrs].
+    destruct s'' as [[[[gps'' mem''] regs''] pc''] addrs''].
     unfold Memory.alloc, merge_states, merge_states_mem, merge_memories, CS.state_component.
     intros Hmerge_ifaces Hdomm.
     rewrite unionmE.
@@ -715,7 +725,7 @@ Section Mergeable.
     destruct (Memory.load (CS.state_mem s) ptr) as [v |] eqn:Hcase1;
       first (symmetry; now apply program_load_to_partialized_memory).
     intros Hpc Hmerge Hptr.
-    destruct s as [[[gps mem] regs] pc]; destruct ptr as [[C b] o];
+    destruct s as [[[[gps mem] regs] pc] addrs]; destruct ptr as [[C b] o];
       unfold Memory.load, merge_memories in *; simpl in *; subst.
     eapply is_program_component_pc_in_domm in Hpc; last eassumption; try assumption.
     inversion Hmerge as [_ _ _ _ _ _ _ Hmergeable_ifaces _ _ _ _ _ _ _ _].
@@ -803,7 +813,7 @@ Section Mergeable.
     find_label_in_procedure (globalenv sem) (CS.state_pc s) l = Some pc ->
     find_label_in_procedure (globalenv sem') (CS.state_pc s) l = Some pc.
   Proof.
-    destruct s as [[[? ?] ?] pc_]. simpl.
+    destruct s as [[[[? ?] ?] pc_] ?]. simpl.
     intros Hpc Hmerge Hlabel.
     inversion Hmerge as [_ _ _ Hwfp Hwfc _ Hwfc' Hmergeable_ifaces _ Hifacec _ _ _ _ _ _].
     pose proof proj1 Hmergeable_ifaces as Hlinkable.
@@ -830,7 +840,7 @@ Section Mergeable.
   Proof.
     intros Hcomp Hmerge.
     unfold CS.is_program_component, CS.is_context_component, CS.state_turn, turn_of in Hcomp.
-    destruct s as [[[gps1 mem1] regs1] pc1].
+    destruct s as [[[[gps1 mem1] regs1] pc1] addrs1].
     inversion Hmerge as [s0 _ t Hwfp Hwfc _ _ Hmergeable_ifaces _ _ Hprog_is_closed _ Hini _ Hstar _].
     destruct (CS.star_pc_domm _ _ Hwfp Hwfc Hmergeable_ifaces Hprog_is_closed Hini Hstar) as [Hip | Hic].
     - assumption.
@@ -936,6 +946,11 @@ Section MergeSym.
       assumption.
   Qed.
 
+  Lemma merge_addrs_sym addrs addrs'' :
+    mergeable_interfaces ip ic ->
+    merge_addrs addrs addrs'' = merge_addrs addrs'' addrs.
+  Admitted.
+
   (* JT: TODO: Clean this proof (RB: agreed). *)
   Theorem merge_states_sym s s'' :
     mergeable_states p c p' c' s s'' ->
@@ -964,24 +979,25 @@ Section MergeSym.
       pose proof linking_well_formedness Hwfp' Hwfc' (proj1 Hmergeable_ifacesC) as Hwf''.
       now exists prog'', s0'', t.
     }
-    destruct s as [[[stack mem] reg] pc]; destruct s'' as [[[stack'' mem''] reg''] pc''].
+    destruct s as [[[[stack mem] reg] pc] addrs]; destruct s'' as [[[[stack'' mem''] reg''] pc''] addrs''].
     unfold merge_states.
     rewrite (merge_stacks_sym Hmergeable_ifaces).
     rewrite (merge_memories_sym Hmergeable_ifaces Hmem Hmem'').
     erewrite (merge_registers_sym _ _ Hmergeable_ifaces).
     rewrite (merge_pc_sym Hmergeable_ifaces).
+    rewrite (merge_addrs_sym _ _ Hmergeable_ifaces).
     reflexivity.
     simpl.
     pose proof CS.star_pc_domm _ _ Hwfp Hwfc Hmergeable_ifaces Hprog_is_closed Hini Hstar as Hdomm.
     rewrite domm_union. now apply /fsetUP.
-    replace pc with (CS.state_pc (stack, mem, reg, pc)); try reflexivity.
-    replace pc'' with (CS.state_pc (stack'', mem'', reg'', pc'')); try reflexivity.
+    replace pc with (CS.state_pc (stack, mem, reg, pc, addrs)); try reflexivity.
+    replace pc'' with (CS.state_pc (stack'', mem'', reg'', pc'', addrs'')); try reflexivity.
     eapply mergeable_states_pc_same_component; eassumption.
     simpl.
     pose proof CS.star_pc_domm _ _ Hwfp Hwfc Hmergeable_ifaces Hprog_is_closed Hini Hstar as Hdomm.
     rewrite domm_union. now apply /fsetUP.
-    replace pc with (CS.state_pc (stack, mem, reg, pc)); try reflexivity.
-    replace pc'' with (CS.state_pc (stack'', mem'', reg'', pc'')); try reflexivity.
+    replace pc with (CS.state_pc (stack, mem, reg, pc, addrs)); try reflexivity.
+    replace pc'' with (CS.state_pc (stack'', mem'', reg'', pc'', addrs'')); try reflexivity.
     eapply mergeable_states_pc_same_component; eassumption.
     eapply mergeable_states_mergeable_stack with (p' := p') (c' := c'); eassumption.
   Qed.
@@ -1098,9 +1114,9 @@ Section ThreewayMultisem1.
       symmetry in Ht12; apply Eapp_E0_inv in Ht12 as [? ?]; subst.
       specialize (IHstar'' Hmerge1 eq_refl). rewrite IHstar''.
       apply star_iff_starR in Hstar12''.
-      destruct s as [[[gps mem] regs] pc].
-      destruct s2'' as [[[gps2'' mem2''] regs2''] pc2''].
-      destruct s3'' as [[[gps3'' mem3''] regs3''] pc3''].
+      destruct s as [[[[gps mem] regs] pc] addrs].
+      destruct s2'' as [[[[gps2'' mem2''] regs2''] pc2''] addrs2''].
+      destruct s3'' as [[[[gps3'' mem3''] regs3''] pc3''] addrs3''].
       inversion Hstep23''; subst;
         (* Unfold, common rewrite on PC, memory rewrite for memory goals and done. *)
         unfold merge_states, merge_registers, merge_pcs, merge_memories, ip;
@@ -1190,9 +1206,9 @@ Section ThreewayMultisem1.
     pose proof threeway_multisem_mergeable_step_E0 Hcomp1 Hmerge1 Hstep12
       as Hmerge2.
     rewrite (mergeable_states_merge_program Hcomp2 Hmerge2).
-    destruct s1 as [[[gps1 mem1] regs1] pc1].
-    destruct s2 as [[[gps2 mem2] regs2] pc2].
-    destruct s1'' as [[[gps1'' mem1''] regs1''] pc1''].
+    destruct s1 as [[[[gps1 mem1] regs1] pc1] addrs1].
+    destruct s2 as [[[[gps2 mem2] regs2] pc2] addrs2].
+    destruct s1'' as [[[[gps1'' mem1''] regs1''] pc1''] addrs1''].
     (* Case analysis on step. *)
     inversion Hstep12; subst;
       t_threeway_multisem_step_E0.
@@ -1294,10 +1310,10 @@ Section ThreewayMultisem1.
     rewrite (mergeable_states_merge_program Hcomp1 Hmerge1).
     pose proof threeway_multisem_event_lockstep_program_mergeable
          Hcomp1 Hmerge1 Hstep12 Hstep12'' as Hmerge2.
-    set s1copy := s1. destruct s1 as [[[gps1 mem1] regs1] pc1].
-    set s2copy := s2. destruct s2 as [[[gps2 mem2] regs2] pc2].
-    destruct s1'' as [[[gps1'' mem1''] regs1''] pc1''].
-    destruct s2'' as [[[gps2'' mem2''] regs2''] pc2''].
+    set s1copy := s1. destruct s1 as [[[[gps1 mem1] regs1] pc1] addrs1].
+    set s2copy := s2. destruct s2 as [[[[gps2 mem2] regs2] pc2] addrs2].
+    destruct s1'' as [[[[gps1'' mem1''] regs1''] pc1''] addrs1''].
+    destruct s2'' as [[[[gps2'' mem2''] regs2''] pc2''] addrs2''].
     (* Case analysis on step. *)
     inversion Hstep12; subst;
       inversion Hstep12''; subst.
@@ -1455,7 +1471,7 @@ Section ThreewayMultisem2.
       apply H; try assumption.
       + unfold CS.is_program_component, CS.is_context_component, turn_of, CS.state_turn.
         pose proof mergeable_states_pc_same_component Hmerge1 as Hpc.
-        destruct s1 as [[[? ?] ?] pc1]; destruct s1'' as [[[? ?] ?] pc1''].
+        destruct s1 as [[[[? ?] ?] pc1] ?]; destruct s1'' as [[[[? ?] ?] pc1''] ?].
         simpl in Hpc.
         rewrite -Hpc.
         unfold CS.is_program_component, CS.is_context_component, turn_of, CS.state_turn in Hcase.
@@ -1654,8 +1670,8 @@ Section ThreewayMultisem3.
   Proof.
     intros Hpc Hmerge Hstep.
     inversion Hmerge as [_ _ _ Hwfp Hwfc Hwfp' Hwfc' Hmergeable_ifaces Hifacep Hifacec _ _ _ _ _ _].
-    destruct s1 as [[[gps1 mem1] regs1] pc1].
-    destruct s1'' as [[[gps1'' mem1''] regs1''] pc1''].
+    destruct s1 as [[[[gps1 mem1] regs1] pc1] addrs1].
+    destruct s1'' as [[[[gps1'' mem1''] regs1''] pc1''] addrs1''].
     inversion Hmergeable_ifaces as [Hlinkable _].
     pose proof linkable_implies_linkable_mains Hwfp Hwfc Hlinkable as Hmain_linkability.
     assert (Hlinkable' := Hlinkable); rewrite Hifacep Hifacec in Hlinkable'.
@@ -1781,8 +1797,8 @@ Section ThreewayMultisem5.
     final_state sem'' s'' ->
     final_state sem'  (merge_states ip ic s s'').
   Proof.
-    destruct s as [[[gps mem] regs] pc].
-    destruct s'' as [[[gps'' mem''] regs''] pc''].
+    destruct s as [[[[gps mem] regs] pc] addrs].
+    destruct s'' as [[[[gps'' mem''] regs''] pc''] addrs''].
     unfold final_state. simpl. unfold merge_pcs.
     intros Hmerge Hfinal Hfinal''.
     inversion Hmerge as [_ _ _ Hwfp Hwfc Hwfp' Hwfc' Hmergeable_ifaces Hifacep Hifacec _ _ _ _ _ _].
@@ -1815,8 +1831,8 @@ Section ThreewayMultisem5.
     ~ final_state sem'' s'' ->
     ~ final_state sem'  (merge_states ip ic s s'').
   Proof.
-    destruct s as [[[gps mem] regs] pc].
-    destruct s'' as [[[gps'' mem''] regs''] pc''].
+    destruct s as [[[[gps mem] regs] pc] addrs].
+    destruct s'' as [[[[gps'' mem''] regs''] pc''] addrs''].
     unfold final_state. simpl. unfold merge_pcs.
     intros Hmerge Hfinal Hfinal'' Hfinal'.
     inversion Hmerge as [_ _ _ Hwfp Hwfc Hwfp' Hwfc' Hmergeable_ifaces Hifacep Hifacec _ _ _ _ _ _ ].
